Replace readlink with stat

examples/sgx/Interpreter.fst
@@ -212,6 +212,20 @@ let ustar buf calltable base wbmapstart uheapstart ustackstart ucodestart entry 
   let stmtlist = mem.decode myprogram entry in
   steps (Mkcpuregstate regslist) mem  myprogram stmtlist
 
+val main:unit -> STL cpuregstate
+	(requires (fun h-> True))
+	(ensures (fun h0 r h1 -> True))
+let main _ = 
+  let base = 1000uL in
+  let wbmapstart = 1100uL in
+  let ucodestart = 1200uL in
+  let ustackstart = 1300uL in
+  let uheapstart = 1400uL in
+  let entry = 1200uL in 
+  let buf = Buffer.create 0uL 500ul in
+  let calltable = Buffer.create 0uL 100ul in
+  let myprogram = [("main", Seq [(Load ((Register "rax"), 4uL, (Register "rbx")))])] in
+  ustar buf calltable base wbmapstart uheapstart ustackstart ucodestart entry myprogram
 
 (* Place holder for parsing manifest and getting the start addresses and  
   calltable
